code/poly1305/Hacl.Poly1305_256.fsti
@@ -19,5 +19,3 @@ val poly1305_update1: poly1305_update1_st M256
 val poly1305_update: poly1305_update_st M256
 
 val poly1305_finish: poly1305_finish_st M256
-
-val mac: poly1305_mac_st M256
