code/poly1305/Hacl.Poly1305_32.fsti
@@ -18,5 +18,3 @@ val poly1305_update1: poly1305_update1_st M32
 val poly1305_update: poly1305_update_st M32
 
 val poly1305_finish: poly1305_finish_st M32
-
-val mac: poly1305_mac_st M32
