code/streaming/Hacl.Streaming.Poly1305_32.fsti
@@ -1,0 +1,27 @@
+module Hacl.Streaming.Poly1305_32
+
+module G = FStar.Ghost
+module F = Hacl.Streaming.Functor
+module I = Hacl.Streaming.Interface
+
+open Hacl.Impl.Poly1305.Fields
+open Hacl.Streaming.Poly1305
+
+#set-options "--fuel 0 --ifuel 0 --z3rlimit 100"
+
+/// Type abbreviation - makes KaRaMeL use pretty names in the generated code
+let state_t = F.state_s (poly1305 M32) () (t M32) (k.I.s ())
+
+noextract
+let alloca = F.alloca (poly1305 M32) () (t M32) (k.I.s ())
+let malloc = F.malloc (poly1305 M32) () (t M32) (k.I.s ())
+let reset = F.reset (poly1305 M32) (G.hide ()) (t M32) (k.I.s ())
+[@@ Comment "0 = success, 1 = max length exceeded" ]
+let update = F.update (poly1305 M32) (G.hide ()) (t M32) (k.I.s ())
+let digest = F.digest (poly1305 M32) () (t M32) (k.I.s ())
+let free = F.free (poly1305 M32) (G.hide ()) (t M32) (k.I.s ())
+
+open Hacl.Impl.Poly1305
+
+(* The one-shot MAC *)
+val mac: poly1305_mac_st M32
