providers/evercrypt/fst/EverCrypt.Poly1305.fst
@@ -130,14 +130,14 @@ let mac output input input_len key =
   let vec128 = EverCrypt.AutoConfig2.has_vec128 () in
 
   if EverCrypt.TargetConfig.hacl_can_compile_vec256 && vec256 then begin
-    Hacl.Poly1305_256.mac output input input_len key
+    Hacl.Streaming.Poly1305_256.mac output input input_len key
 
   end else if EverCrypt.TargetConfig.hacl_can_compile_vec128 && vec128 then begin
-    Hacl.Poly1305_128.mac output input input_len key
+    Hacl.Streaming.Poly1305_128.mac output input input_len key
 
   end else if EverCrypt.TargetConfig.hacl_can_compile_vale then begin
     poly1305_vale output input input_len key
 
   end else begin
-    Hacl.Poly1305_32.mac output input input_len key
+    Hacl.Streaming.Poly1305_32.mac output input input_len key
   end
